big code restructuring

proof/schnorr_protocol/leakage_freeness/Challenge_LF.ec
@@ -3,14 +3,54 @@ require import List Int AllCore Distr.
 from Jasmin require import JModel.
 
 require import AuxLemmas.
-require import Ops_LeakageFunctions.
+require import BigNum_LF.
+require import Random_bit_LF.
 
 
 require import W64_SchnorrExtract_ct.
 module M1 = W64_SchnorrExtract_ct.M(W64_SchnorrExtract_ct.Syscall).
 
 
+(* challenge LEAKAGES  *)
+op challenge_t : leakages_t = uniform_binary_choice_t ++
+ [LeakAddr []] ++ set1_f 32 ++ [LeakAddr []] ++ set0_f 32 ++ [LeakAddr []].
+
+lemma challenge_leakages start_l : 
+  hoare [ M(Syscall).challenge : M.leakages = start_l ==> M.leakages = challenge_t ++ start_l].
+proc.
+pose suf1 :=  [LeakAddr []] ++ start_l.
+seq 6 : (M.leakages = set0_f 32 ++ suf1 ).
+wp.  call (bn_set0_leakages suf1). simplify. wp. skip. progress. auto.
+pose suf2 :=  [LeakAddr []] ++ set0_f 32 ++ suf1.
+seq 3 : (M.leakages = set1_f 32 ++ suf2).
+wp.  call (bn_set1_leakages suf2). wp. skip. progress.
+pose suf3 :=  [LeakAddr []] ++ set1_f 32 ++ suf2.
+seq 3 : (M.leakages = uniform_binary_choice_t ++ suf3).
+call (uniform_binary_choice_leakages suf3). wp. skip. progress.
+skip. progress.
+rewrite /suf3 /suf2 /suf1. 
+do? rewrite - catA. 
+do? rewrite  catA.  auto.
+qed.
+
+
+lemma challenge_ll : 
+  islossless M(Syscall).challenge.
+proc. 
+wp. call uniform_binary_choice_ll. 
+wp. call bn_set1_ll.
+wp. call bn_set0_ll.
+auto.
+qed.
+
 lemma challenge_leakages_ph start_l : 
+  phoare [ M(Syscall).challenge : M.leakages = start_l ==> M.leakages = challenge_t ++ start_l] = 1%r.
+phoare split !  1%r 0%r. auto.
+conseq challenge_ll. hoare. conseq (challenge_leakages start_l).
+qed.
+
+
+lemma challenge_leakages_ph0 start_l : 
   phoare [ M(Syscall).challenge : M.leakages = start_l ==> M.leakages <> challenge_t ++ start_l] = 0%r.
 hoare. simplify.
 apply challenge_leakages.
@@ -33,7 +73,7 @@ progress.
    <= Pr[M(Syscall).challenge() @ &m :  M1.leakages <> challenge_t ].
    rewrite Pr[mu_sub]. smt(). auto.
    have ->: Pr[M(Syscall).challenge() @ &m :  M1.leakages <> challenge_t ] = 0%r.
-   byphoare (_: M.leakages = [] ==> _). conseq (challenge_leakages_ph []). 
+   byphoare (_: M.leakages = [] ==> _). conseq (challenge_leakages_ph0 []). 
    progress. smt(@List).  smt(@List).  auto. auto.
    smt(@Distr). simplify. auto.
  have ->: Pr[M(Syscall).challenge() @ &m : res = a /\ M.leakages = challenge_t] 
@@ -45,7 +85,7 @@ progress.
     Pr[M(Syscall).challenge() @ &m : M.leakages = l /\ res = a /\ M.leakages <> challenge_t].
  rewrite Pr[mu_eq]. smt(). auto.
  have fact2 : Pr[M(Syscall).challenge() @ &m : M.leakages = l /\ res = a /\ M.leakages <> challenge_t] = 0%r.
-  byphoare (_: M.leakages = [] ==> _). proc*. call (challenge_leakages_ph []). skip. progress. 
+  byphoare (_: M.leakages = [] ==> _). proc*. call (challenge_leakages_ph0 []). skip. progress. 
   smt(@List). auto. auto. 
   smt().
 qed.
