proof/modular_multiplication/leakage_freeness/BarretReduction_Concrete_CT.ec
@@ -1,0 +1,82 @@
+require import List Int AllCore. 
+require import W64_SchnorrExtract_ct.
+from Jasmin require import JModel.
+
+require import BigNum_LF.
+
+(* bn_breduce LEAKAGES  *)
+op bn_breduce_f : leakages_t = bn_shrink_f 32 ++
+[LeakAddr []] ++ dcminusP_f ++
+[LeakAddr []] ++ bn_expand_f 32 ++
+[LeakAddr []] ++ dsub_f 64 ++
+[LeakAddr []; LeakAddr []; LeakAddr []] ++ bn_muln_f 32 ++
+[LeakAddr []; LeakAddr []] ++ bn_shrink_f 32 ++
+[LeakAddr []] ++ div2_f 64 64 ++
+[LeakAddr []] ++ dbn_muln_f 64 ++ [LeakAddr []; LeakAddr []].
+
+lemma bn_breduce_leakages start_l :
+   hoare [ M(Syscall).bn_breduce : M.leakages = start_l 
+     ==> M.leakages = bn_breduce_f ++ start_l ].
+proof. 
+proc. 
+pose suf1 :=  [LeakAddr []; LeakAddr []] ++ start_l.
+seq 16 : (M.leakages = dbn_muln_f 64 ++ suf1 ).
+wp.  call (dbn_muln_leakages suf1). simplify. wp. skip. progress. 
+
+pose suf2 :=  [LeakAddr []] ++ dbn_muln_f 64 ++ suf1.
+seq 6 : (M.leakages = div2_f 64 64 ++ suf2).
+wp.  call (div2_leakages suf2 64). simplify. wp. skip. progress. 
+
+pose suf3 :=  [LeakAddr []] ++ div2_f 64 64 ++ suf2.
+seq 3 : (M.leakages = bn_shrink_f 32 ++ suf3).
+wp.  call (bn_shrink_leakages suf3). simplify. wp. skip. progress. 
+
+pose suf4 :=  [LeakAddr [] ;  LeakAddr []] ++ bn_shrink_f 32 ++ suf3.
+seq 9 : (M.leakages = bn_muln_f 32 ++ suf4).
+wp.  call (bn_muln_leakages suf4). simplify. wp. skip. progress.  rewrite /suf4.
+
+pose suf5 :=  [LeakAddr [];LeakAddr [];LeakAddr []] ++ bn_muln_f 32 ++ suf4.
+seq 9 : (M.leakages = dsub_f 64  ++ suf5).
+wp.  call (dbn_subc_leakages suf5). simplify. wp. skip. progress. 
+
+pose suf6 :=  [LeakAddr []] ++ dsub_f 64 ++ suf5.
+seq 4 : (M.leakages = bn_expand_f 32  ++ suf6).
+wp. call (bn_expand_leakages suf6). simplify. wp. skip. progress. 
+
+pose suf7 :=  [LeakAddr []] ++ bn_expand_f 32 ++ suf6.
+seq 3 : (M.leakages = dcminusP_f   ++ suf7).
+wp. call (dcminusP_leakages suf7). simplify. wp. skip. progress. 
+
+pose suf8 :=  [LeakAddr []] ++ dcminusP_f ++ suf7.
+seq 4 : (M.leakages = bn_shrink_f 32   ++ suf8).
+wp. call (bn_shrink_leakages suf8). wp. skip.
+progress.
+skip. progress.
+rewrite /suf8 /suf7 /suf6 /suf5 /suf4 /suf3 /suf2 /suf1.
+rewrite /bn_breduce_f. 
+do ? rewrite catA. auto.
+qed.
+
+
+lemma bn_breduce_ll : islossless M(Syscall).bn_breduce.
+proc.
+wp. call bn_shrink_ll.
+wp. call dcminusP_ll. 
+wp. call bn_expand_ll.
+wp. call dbn_subc_ll.
+wp. call bn_muln_ll.
+wp. call bn_shrink_ll.
+wp. call div2_ll. simplify.
+wp. call dbn_muln_ll.
+wp. auto.
+qed.
+
+
+lemma bn_breduce_leakages_ph start_l :
+   phoare [ M(Syscall).bn_breduce : M.leakages = start_l 
+     ==> M.leakages = bn_breduce_f ++ start_l ] = 1%r.
+phoare split !  1%r 0%r. auto.
+conseq bn_breduce_ll. hoare. conseq (bn_breduce_leakages start_l).
+qed.
+
+
