proof/modular_multiplication/leakage_freeness/ModularMultiplication_Concrete_CT.ec
@@ -1,0 +1,44 @@
+require import List Int AllCore. 
+require import W64_SchnorrExtract_ct.
+from Jasmin require import JModel.
+
+require import BigNum_LF.
+require import BarretReduction_Concrete_CT.
+
+(* mulm LEAKAGES  *)
+op [opaque] mulm_t : leakages_t = bn_breduce_f ++ [LeakAddr []] ++ bn_muln_f 32  ++
+[LeakAddr []; LeakAddr [] ; LeakAddr []] .
+lemma mulm_leakages start_l :
+   hoare [ M(Syscall).bn_mulm : M.leakages = start_l
+                ==> M.leakages = mulm_t ++ start_l ].
+proof. proc.
+pose suf1 :=  [LeakAddr [];LeakAddr []; LeakAddr []] ++ start_l.
+seq 11 : (M.leakages = bn_muln_f 32 ++ suf1 ).
+wp. call (bn_muln_leakages suf1). simplify. wp. skip. progress.
+
+pose suf2 :=  [LeakAddr []] ++ bn_muln_f 32 ++ suf1.
+seq 7 : (M.leakages = bn_breduce_f ++ suf2).
+wp. call (bn_breduce_leakages suf2). simplify. wp. skip. progress.
+skip. auto.
+progress.
+rewrite /suf2 /suf1.
+rewrite /mulm_t /bn_muln_f.
+do? rewrite catA. auto.
+qed.
+
+lemma bn_mulm_ll : islossless M(Syscall).bn_mulm.
+proc.
+wp. call bn_breduce_ll.
+wp. call bn_muln_ll.
+wp. auto.
+qed.
+
+
+lemma bn_mulm_leakages_ph start_l :
+   phoare [ M(Syscall).bn_mulm : M.leakages = start_l
+     ==> M.leakages = mulm_t ++ start_l ] = 1%r.
+phoare split !  1%r 0%r. auto.
+conseq bn_mulm_ll. hoare. conseq (mulm_leakages start_l).
+qed.
+
+
