proof/random_bit/Random_bit_proof.ec
@@ -5,7 +5,7 @@ from Jasmin require import JModel.
 require import Array32.
 require BinUniSample_spec.
 require import Array1 WArray1.
-require import Finite FinLists.
+require import Finite ArrayFiniteness.
 
 require import BigNum_proofs.
 require import W64_SchnorrExtract.
