proof/random_bit/leakage_freeness/Random_bit_LF.ec
@@ -1,0 +1,72 @@
+require import List Int AllCore Distr.
+from Jasmin require import JModel.
+
+require import AuxLemmas.
+require import BigNum_LF.
+
+
+require import W64_SchnorrExtract_ct.
+module M1 = W64_SchnorrExtract_ct.M(W64_SchnorrExtract_ct.Syscall).
+
+(* random_bit LEAKAGES  *)
+op random_bit_t : leakages_t =  LeakAddr [] ::  LeakAddr [0] :: LeakAddr [] :: LeakAddr [] :: [].
+
+lemma random_bit_leakages start_l : 
+  hoare [ M(Syscall).random_bit : M.leakages = start_l ==> M.leakages = random_bit_t ++ start_l].
+proc. wp. call (_:true). rnd. skip. progress.
+wp. skip. progress. 
+qed.
+
+lemma random_bit_ll : islossless M(Syscall).random_bit.
+proc. inline*. wp. rnd. wp. skip.
+progress. 
+apply dmap_ll.
+apply dmap_ll.
+apply  DList.dlist_ll. smt(@W8).
+qed.
+
+
+lemma random_bit_leakages_ph start_l :
+  phoare [ M(Syscall).random_bit : M.leakages = start_l 
+            ==> M.leakages = random_bit_t ++ start_l ] = 1%r.
+phoare split !  1%r 0%r. auto.
+conseq random_bit_ll. hoare. conseq (random_bit_leakages start_l).
+qed.
+
+
+(* uniform_binary_choice LEAKAGES  *)
+
+op uniform_binary_choice_t : leakages_t = bn_cmov_f 32 ++
+[LeakAddr []; LeakAddr []] ++ random_bit_t ++ LeakAddr [] :: [].
+
+lemma uniform_binary_choice_leakages start_l : 
+  hoare [ M(Syscall).uniform_binary_choice : M.leakages = start_l 
+    ==> M.leakages = uniform_binary_choice_t ++ start_l].
+proc.
+pose suf1 :=  [LeakAddr []] ++ start_l.
+seq 3 : (M.leakages = random_bit_t ++ suf1 ).
+wp.  call (random_bit_leakages suf1).  wp.  skip. progress. 
+pose suf2 :=  [LeakAddr []; LeakAddr []] ++ random_bit_t ++ suf1.
+seq 6 : (M.leakages = bn_cmov_f 32 ++ suf2 ).
+wp.  call (bn_cmov_leakages suf2).  wp.  skip. progress.  
+rewrite /suf2 /suf1. 
+skip. progress.
+rewrite /uniform_binary_choice_t. 
+do? rewrite - catA. simplify. 
+do? rewrite  catA.  auto.
+qed.
+
+lemma uniform_binary_choice_ll : 
+  islossless M(Syscall).uniform_binary_choice.
+proc. 
+wp. call bn_cmov_ll. 
+wp. call random_bit_ll.
+auto.
+qed.
+
+lemma uniform_binary_choice_leakages_ph start_l : 
+  phoare [ M(Syscall).uniform_binary_choice : M.leakages = start_l 
+    ==> M.leakages = uniform_binary_choice_t ++ start_l] = 1%r.
+phoare split !  1%r 0%r. auto.
+conseq uniform_binary_choice_ll. hoare. conseq (uniform_binary_choice_leakages start_l).
+qed.
