proof/rejection_sampling/leakage_freeness/UniformSampling_Concrete_LeakagesFun.ec
@@ -1,0 +1,131 @@
+require import List Int AllCore. 
+require import W64_SchnorrExtract_ct.
+from Jasmin require import JModel.
+
+require import BigNum_LF.
+
+
+op samp_prefix : leakages_t =
+  LeakCond (! set0_64_.`2) :: LeakAddr [] :: LeakAddr [] :: (set0_f 32 ++
+                                                           [LeakAddr [];
+                                                              LeakAddr []]).
+op samp_step  : leakages_t = LeakCond true :: LeakAddr [] :: LeakAddr [] :: (sub_f 32 ++
+                                                LeakAddr [] :: (copy_f 32 ++
+                                                                LeakAddr [] :: LeakAddr [] ::
+                                                                LeakAddr [] :: [])) .
+
+
+op samp_g (x : int) : leakages_t = if (x < 0) then [(LeakAddr [x])] else iteri x (fun i r => samp_step  ++ r) [].
+lemma samp_g_comp_1 x : x = 0 => samp_g x = [].  rewrite /samp_g.
+smt(@Int). qed.
+lemma samp_g_comp_2 x : 0 <  x  => samp_g x = samp_step  ++ samp_g (x - 1).
+rewrite /samp_g. move => q.
+have ->: x < 0 = false. smt().
+have ->: x - 1 < 0 = false. smt(). simplify.
+smt(@Int). qed.
+
+
+op samp_suffix : leakages_t =
+ LeakCond false :: LeakAddr [] :: LeakAddr []
+   :: (sub_f 32 ++ LeakAddr [] ::
+      (copy_f 32 ++ LeakAddr [] :: LeakAddr [] :: LeakAddr [] :: [])).
+
+op samp_f (x : int) : leakages_t = samp_g x ++ samp_prefix.
+op samp_t (x : int) : leakages_t = samp_suffix ++ samp_f (x - 1).
+
+lemma samp_t_inj : injective samp_t.
+
+ have fact1 : size (samp_t 1)  = size samp_suffix + size samp_prefix.
+  rewrite /samp_t. rewrite /samp_f. simplify. rewrite samp_g_comp_1.   auto. simplify.
+  rewrite size_cat. simplify.
+  smt(@Int).
+
+ have fact2 : forall x, x <= 0 => size (samp_t x) = 1 + size samp_suffix + size samp_prefix.
+  progress.  rewrite /samp_t.
+  rewrite /samp_f /samp_g.
+  have ->: x - 1 < 0. smt(). simplify.
+  rewrite size_cat. simplify.
+   smt(@Int).
+  
+
+ have fact3 : forall x, 0 <= x => size (samp_g x) = x * (size samp_step).
+   apply intind. progress.
+    rewrite /samp_f /samp_prefix. rewrite samp_g_comp_1. auto. auto.
+   progress.
+    rewrite samp_g_comp_2. smt().
+    rewrite size_cat. simplify. smt(@Int).
+ 
+ have fact4: forall x, 1 <= x => size (samp_t x) = (x - 1) * (size samp_step) + size samp_suffix + size samp_prefix . progress. rewrite /samp_t. rewrite size_cat. rewrite /samp_f.
+   rewrite size_cat. rewrite fact3. smt(). smt(@Int).
+
+ have fact5 : 1 <= size samp_step. rewrite /samp_step. simplify. smt(@List).
+ clear fact3.
+    
+ have fact6 : forall x y, x <> y => samp_t x <> samp_t y.
+  move => x y xneqy.
+    case (x <= 0) => xh.
+    case (y <= 0) => yh.
+    rewrite /samp_t. rewrite /samp_f.  rewrite /samp_f. rewrite /samp_g.
+     have ->: x - 1 < 0 = true. smt().
+     have ->: y - 1 < 0 = true. smt().
+    simplify.
+     smt(@List).
+
+  rewrite /samp_t. rewrite /samp_f. rewrite /samp_g.
+     have ->: x - 1 < 0 = true. smt().
+     have ->: y - 1 < 0 = false. smt(). simplify.
+     case (y - 1 = 0) => y0. rewrite iteri0. smt(). simplify. smt(@List).
+     rewrite iteri_red. smt(). simplify. rewrite /samp_step. smt(@List).
+
+  case (y <= 0) => yh.
+  rewrite /samp_t. rewrite /samp_f. rewrite /samp_g.
+     have ->: x - 1 < 0 = false. smt().
+     have ->: y - 1 < 0 = true. smt(). simplify.
+     case (x - 1 = 0) => x0. rewrite iteri0. smt(). simplify. smt(@List).
+     rewrite iteri_red. smt(). simplify. rewrite /samp_step. smt(@List).
+
+  have : size (samp_t x) <> size (samp_t y).
+   rewrite fact4. smt().
+   rewrite fact4. smt().
+  smt(@Int).
+  smt().
+smt().
+qed.
+
+
+
+
+lemma rsample_leakages l :
+  hoare [ M(Syscall).bn_rsample : M.leakages = l
+     ==> M.leakages = samp_t res.`1 ++ l].
+proc.
+seq 18 :  (M.leakages = samp_prefix ++ l /\ i = 0  /\ cf = false ).
+wp. ecall (bn_set0_leakages M.leakages). wp. skip. progress.
+rewrite /samp_prefix. simplify. smt(@List).
+while (0 <= i /\ (cf = false => M.leakages = samp_f i ++ l)
+              /\ (cf = true => M.leakages = samp_t i ++ l)).
+wp.  ecall (bn_subc_leakages M.leakages). simplify.
+wp.  ecall (bn_copy_leakages M.leakages). simplify.
+wp. inline Syscall.randombytes_256. wp. rnd.  wp.
+skip. progress. smt().  rewrite H4.  rewrite H0. rewrite H2. auto. simplify.
+rewrite /samp_f. rewrite (samp_g_comp_2 (i{hr} + 1)). smt().
+simplify.
+rewrite /samp_step. simplify.
+have ->: (copy_f 32 ++
+                LeakAddr [] :: LeakAddr [] :: LeakAddr [] :: (samp_g i{hr} ++ samp_prefix ++
+                                               l))
+ = (copy_f 32 ++ [LeakAddr [] ; LeakAddr []; LeakAddr []]) ++
+samp_g i{hr} ++ samp_prefix ++ l.
+do ? rewrite - catA. simplify. auto.
+smt(@List).
+rewrite /samp_t. simplify.
+rewrite /samp_suffix.  simplify.  split. rewrite H4. auto.
+rewrite H0. rewrite H2. auto.
+do ? rewrite - catA. simplify.
+congr. congr. congr.
+do ? rewrite - catA. congr. simplify. auto.
+skip. progress. rewrite /samp_prefix. rewrite /samp_f. rewrite samp_g_comp_1.
+auto. rewrite /samp_prefix. auto.
+rewrite H2. rewrite H. auto.
+auto.
+qed.
